some library refactoring, reduce deps

src/lib/kuiper/Kuiper.Base.fsti
@@ -2,12 +2,11 @@ module Kuiper.Base
 
 #lang-pulse
 
-open Pulse.Lib.Pervasives
-open FStar.Tactics.V2
-open FStar.Seq
-open Pulse.Lib.BigStar
+open Kuiper.Common
 open Kuiper.SizeT
-open FStar.Mul
+open FStar.Ghost
+open Pulse.Lib.Core
+open Pulse.Main
 module SZ = FStar.SizeT
 
 type mode_t = | CPU | GPU
@@ -81,27 +80,3 @@ fn thread_idx_x () (#n: tid_t)
   requires  emp
   returns   id : SZ.t
   ensures   pure (SZ.v id == tidx_x n)
-
-let lemma_mul_lt (a b: nat) (c: nat { a < c }) (d: nat { b <= d /\ d > 0 }): Lemma (a * b < c * d) = ()
-
-noextract inline_for_extraction
-fn thread_idx_all () (#n: tid_t)
-  preserves
-    thread_id n
-  requires
-    emp
-  returns
-    id : SZ.t
-  ensures
-    pure (SZ.v id == thread_index n /\ SZ.v id < max_blocks * max_threads)
-{
-  assert (pure (bidx_x n < 1024 * 1024 * 1024 /\ tidx_x n < 1024 /\ bdim_x n <= 1024));
-  lemma_mul_lt (bidx_x n) (bdim_x n) (1024 * 1024 * 1024) 1024;
-  assert (pure (bidx_x n * tidx_x n < 1024 * 1024 * 1024 * 1024 /\ bdim_x n <= 1024));
-  let bid = block_idx_x ();
-  let bdim = block_dim_x ();
-  let tid = thread_idx_x ();
-  open FStar.SizeT;
-  let r = (bid *^ bdim) +^ tid;
-  r
-}
